\documentclass[12pt,a4paper]{article}
\usepackage[english,german]{babel}
\usepackage[utf8]{inputenc}
\usepackage{color}
\usepackage{hyperref}
\usepackage{mathtools}
%\usepackage{amsmath}
\usepackage{graphicx}
\usepackage{cancel}
\usepackage{geometry}
\geometry{
  left=3cm,
  right=3cm,
  top=3cm,
  bottom=4cm,
  bindingoffset=5mm
}

\setlength{\parindent}{0em} 
\hypersetup{
    colorlinks=true,
    linktoc=all,
    linkcolor=black,
    urlcolor=black
}
%Gummi|065|=)
%\title{\Huge\textbf{Praktikum Verhaltensneurogenetik}}
\title{\Huge\textbf{$<$Titel$>$}}
\author{Alexander Scholz}
\date{$<$Datum$>$}

% set title of table of contents
\renewcommand*\contentsname{Inhalt}

% https://www.sharelatex.com/learn
% http://www.math.ubc.ca/~cautis/tools/latexmath.html
% http://www.golatex.de/wiki/Kategorie:Befehlsreferenz
% https://en.wikibooks.org/wiki/LaTeX/Mathematics

\begin{document}

\begin{titlepage}

\maketitle
\thispagestyle{empty}
\end{titlepage}

$|\sum \limits_{i=1}^{k}i - \sum \limits_{i=k+1}^{n}i|$ â€¦mit n=2k, $k\in N$\\
$$= \sum \limits_{i=k+1}^{n}i - \sum \limits_{i=1}^{k}i = \sum \limits_{i=1}^{k+1}i+k+1 - \sum \limits_{i=1}^{k}i = \sum \limits_{i=1}^{k}i+k - \sum \limits_{i=1}^{k}i = \sum \limits_{i=1}^{k} (i+k) -1$$
$$= \sum \limits_{i=1}^{k} k = k \cdot k = k^2$$

Beispiel:\\
$$k=2 : \sum \limits_{i=3}^{4} i - \sum \limits_{i=1}^{2} i= 2^2 = 4$$
$$k=2 : \sum \limits_{i=4}^{6} i - \sum \limits_{i=1}^{3} i= 3^2 = 9$$

\end{document}